template-coq/theories/WfInv.v
@@ -1,6 +1,6 @@
 (* Distributed under the terms of the MIT license. *)
 From Coq Require Import ssreflect ssrbool.
-From MetaCoq.Template Require Import config utils Ast AstUtils.
+From MetaCoq.Template Require Import config utils Ast AstUtils Environment.
 
 (** * Inversion lemmas for the well-formedness judgement *)
 
@@ -15,7 +15,7 @@ Fixpoint wf_Inv (t : term) :=
   | tLetIn na t b b' => wf t /\ wf b /\ wf b'
   | tApp t u => isApp t = false /\ u <> nil /\ wf t /\ Forall wf u
   | tConst _ _ | tInd _ _ | tConstruct _ _ _ => True
-  | tCase ci p c brs => wf p /\ wf c /\ Forall (wf ∘ snd) brs
+  | tCase ci p c brs => Forall wf (pparams p) /\ wf (preturn p) /\ wf c /\ Forall (wf ∘ snd) brs
   | tProj p t => wf t
   | tFix mfix k => Forall (fun def => wf def.(dtype) /\ wf def.(dbody)) mfix
   | tCoFix mfix k => Forall (fun def => wf def.(dtype) /\ wf def.(dbody)) mfix
@@ -70,7 +70,8 @@ Fixpoint wf_term (t : term) : bool :=
   | tLetIn na t b b' => wf_term t && wf_term b && wf_term b'
   | tApp t u => ~~ isApp t && ~~ is_empty u && wf_term t && forallb wf_term u
   | tConst _ _ | tInd _ _ | tConstruct _ _ _ => true
-  | tCase ci p c brs => wf_term p && wf_term c && forallb (wf_term ∘ snd) brs
+  | tCase ci p c brs => forallb wf_term (pparams p) && wf_term (preturn p)
+                        && wf_term c && forallb (wf_term ∘ snd) brs
   | tProj p t => wf_term t
   | tFix mfix k =>
     forallb (fun def => wf_term def.(dtype) && wf_term def.(dbody) && isLambda def.(dbody)) mfix
